clean up

HOL_To_IMP_Minus/Refinements/HOL_To_IMP_Minus_Datatypes.thy
@@ -6,9 +6,6 @@ theory HOL_To_IMP_Minus_Datatypes
 begin
 
 datatype_compile_nat cmp_val
-datatype 'a my_option = None | Some 'a
-datatype_compile_nat my_option
-(* datatype_compile_nat option *) (* ?? *)
 
 locale HOL_To_HOL_Nat =
   notes transport_eq_id.partial_equivalence_rel_equivalenceI[per_intro del]
@@ -47,7 +44,7 @@ section \<open>Option\<close>
 
 paragraph \<open>is_some\<close>
 
-fun is_some :: "'a my_option \<Rightarrow> bool" where
+fun is_some :: "'a option \<Rightarrow> bool" where
   "is_some (Some _) = True" |
   "is_some None = False"
 
@@ -57,7 +54,7 @@ function_compile_nat is_some_eq
 
 paragraph \<open>get_some\<close>
 
-fun get_some :: "'a \<Rightarrow> 'a my_option \<Rightarrow> 'a" where
+fun get_some :: "'a \<Rightarrow> 'a option \<Rightarrow> 'a" where
   "get_some _ (Some x) = x" |
   "get_some d _ = d"
 
@@ -73,20 +70,15 @@ fun length_aux :: "nat \<Rightarrow> 'a list \<Rightarrow> nat" where
   "length_aux acc [] = acc" |
   "length_aux acc (_ # xs) = length_aux (Suc acc) xs"
 
-(* definition length0 :: "'a list \<Rightarrow> nat" where *)
-  (* "length0 = length_aux 0" *)
-
 lemma length_eq_length_aux: "List.length xs + k = length_aux k xs"
   by (induction k xs rule: length_aux.induct) auto
 
-lemma length_eq_length0: "List.length xs = length_aux 0 xs"
-  (* unfolding length0_def *)
+lemma length_eq_length_aux0: "List.length xs = length_aux 0 xs"
   by (rule length_eq_length_aux[where k = 0, simplified])
 
 case_of_simps length_aux_eq : length_aux.simps
 function_compile_nat length_aux_eq
-(* function_compile_nat length0_def *)
-function_compile_nat length_eq_length0
+function_compile_nat length_eq_length_aux0
 
 
 paragraph\<open>compare_lengths\<close>
@@ -101,38 +93,33 @@ case_of_simps compare_lengths_eq : compare_lengths.simps
 function_compile_nat compare_lengths_eq
 
 
-paragraph \<open>rev_append\<close>
+paragraph \<open>rev_aux\<close>
 
-fun rev_append :: "'a list \<Rightarrow> 'a list \<Rightarrow> 'a list" where
-  "rev_append [] acc = acc" |
-  "rev_append (x # xs) acc = rev_append xs (x # acc)"
+fun rev_aux :: "'a list \<Rightarrow> 'a list \<Rightarrow> 'a list" where
+  "rev_aux acc [] = acc" |
+  "rev_aux acc (x # xs) = rev_aux (x # acc) xs"
 
-case_of_simps rev_append_eq : rev_append.simps
-function_compile_nat rev_append_eq
+case_of_simps rev_aux_eq : rev_aux.simps
+function_compile_nat rev_aux_eq
 
 
 paragraph \<open>rev\<close>
 
-definition rev0 :: "'a list \<Rightarrow> 'a list" where
-  "rev0 xs = rev_append xs []"
+lemma rev_eq_rev_aux: "List.rev xs @ ys = local.rev_aux ys xs"
+  by (induction ys xs rule: rev_aux.induct) auto
 
-lemma rev_eq_rev_aux: "List.rev xs @ ys = local.rev_append xs ys"
-  by (induction xs ys rule: rev_append.induct) auto
+lemma rev_eq_rev_aux0: "List.rev = rev_aux []"
+  using rev_eq_rev_aux[where ys = "[]"] by auto
 
-lemma rev_eq_rev0: "List.rev xs = local.rev0 xs"
-  unfolding rev0_def
-  using rev_eq_rev_aux[where ys = "[]"] by simp
-
-function_compile_nat rev0_def
-function_compile_nat rev_eq_rev0
+function_compile_nat rev_eq_rev_aux0
 
 
 paragraph \<open>append\<close>
 
-lemma append_eq_append0: "List.append xs ys = rev_append (rev xs) ys"
+lemma append_eq_rev_aux: "List.append xs ys = rev_aux ys (rev xs)"
   unfolding rev_eq_rev_aux[symmetric] by simp
 
-function_compile_nat append_eq_append0
+function_compile_nat append_eq_rev_aux
 
 
 paragraph \<open>zip\<close>
@@ -144,96 +131,25 @@ fun zip_aux :: "('a \<times> 'b) list \<Rightarrow> 'a list \<Rightarrow> 'b lis
 
 lemma zip_eq_zip_aux: "rev zs @ List.zip xs ys = rev (zip_aux zs xs ys)"
   apply (induction zs xs ys rule: zip_aux.induct)
-  unfolding rev_eq_rev0[symmetric] by auto
+  unfolding rev_eq_rev_aux[symmetric] by auto
 
 lemma zip_eq_zip_aux0: "List.zip xs ys = rev (zip_aux [] xs ys)"
   using zip_eq_zip_aux[where zs = "[]"]
-  unfolding rev_eq_rev0[symmetric] by auto
+  unfolding rev_eq_rev_aux[symmetric] by auto
 
 case_of_simps zip_aux_eq : zip_aux.simps
 function_compile_nat zip_aux_eq
-function_compile_nat zip_eq_zip_aux0 (* slow? *)
+function_compile_nat zip_eq_zip_aux0 (* TODO: this step is quite a bit slower *)
 
 
 subsection \<open>Association Lists\<close>
 
-fun assoc_lookup :: "'k \<Rightarrow> ('k \<times> 'v) list \<Rightarrow> 'v my_option" where
+fun assoc_lookup :: "'k \<Rightarrow> ('k \<times> 'v) list \<Rightarrow> 'v option" where
   "assoc_lookup _ [] = None" |
   "assoc_lookup x ((k, v) # xs) = (if x = k then Some v else assoc_lookup k xs)"
 
 case_of_simps assoc_lookup_eq : assoc_lookup.simps
 function_compile_nat assoc_lookup_eq
-
-(* TODO: assoc_delete, assoc_update *)
-
-subsection \<open>Sorting\<close>
-
-text \<open>Sorting, based on decorate-sort-undecorate. Sorts tuples (nat, 'a) on the nat component.
-  For sorting arbitrary datatypes, they must first be mapped to an integer key, sorted, then
-  the key stripped away. Best we can do, since we cannot write a polymorphic sort.\<close>
-(* TODO: or can we do something with typeclasses? *)
-
-type_synonym 'a sort_key = "(nat \<times> 'a)"
-
-fun insort_deco_aux :: "'a sort_key list \<Rightarrow> 'a sort_key \<Rightarrow> 'a sort_key list \<Rightarrow> 'a sort_key list" where
-  "insort_deco_aux acc k [] = rev (k # acc)" |
-  "insort_deco_aux acc k' (k # xs) =
-    (if fst k' \<le> fst k then rev_append (k' # acc) (k # xs) else insort_deco_aux (k # acc) k' xs)"
-
-case_of_simps insort_deco_aux_eq : insort_deco_aux.simps
-(* function_compile_nat insort_deco_aux_eq *)
-(* this refuses to compile *)
-
-lemma insort_key_fst_eq_insort_deco_aux: "rev acc @ insort_key fst k xs = insort_deco_aux acc k xs"
-  apply (induction acc k xs rule: insort_deco_aux.induct) using rev_eq_rev_aux by auto
-
-definition insort_deco :: "'a sort_key \<Rightarrow> 'a sort_key list \<Rightarrow> 'a sort_key list" where
-  "insort_deco = insort_deco_aux []"
-
-lemma insort_key_fst_eq_insort_deco_aux0: "insort_key fst k xs = insort_deco k xs"
-  unfolding insort_deco_def using insort_key_fst_eq_insort_deco_aux[where acc = "[]", simplified] by fast
-
-(* function_compile_nat insort_deco_def *)
-
-fun sort_deco_aux :: "'a sort_key list \<Rightarrow> 'a sort_key list \<Rightarrow> 'a sort_key list" where
-  "sort_deco_aux acc [] = acc" |
-  "sort_deco_aux acc (x # xs) = sort_deco_aux (insort_deco x acc) xs"
-
-case_of_simps sort_deco_aux_eq : sort_deco_aux.simps
-(* function_compile_nat sort_deco_aux_eq *)
-
-lemma sort_key_eq_sort_deco_aux:
-  assumes sorted_acc: "sorted (map fst acc)" shows "sort_key fst (xs @ acc) = sort_deco_aux acc (rev xs)"
-proof-
-  have "sort_key fst (xs @ acc) = foldl (\<lambda>x y. insort_key fst y x) acc (rev xs)"
-    by (subst sort_key_def, subst foldr_append, subst sort_key_def[symmetric],
-        subst sort_key_id_if_sorted[OF sorted_acc], subst foldr_conv_foldl, rule refl)
-  moreover have "foldl (\<lambda>x y. insort_key fst y x) acc xs = sort_deco_aux acc xs" for xs
-    by (induction xs arbitrary: acc) (auto simp add: insort_key_fst_eq_insort_deco_aux0)
-  ultimately show "sort_key fst (xs @ acc) = sort_deco_aux acc (rev xs)" by simp
-qed
-
-lemma sort_key_eq_sort_deco_aux0: "sort_key fst xs = sort_deco_aux [] (rev xs)"
-  using sort_key_eq_sort_deco_aux[where acc = "[]"] by auto
-
-definition sort_deco :: "'a sort_key list \<Rightarrow> 'a sort_key list" where
-  "sort_deco = sort_deco_aux []"
-
-(* function_compile_nat sort_deco_def *)
-
-(* For sort_deco and helpers it's not really clear how to generate a "drop-in" compilable function
-   compatible with sort, since we can't compile "sort_key fst" to IMP. Thus, code will
-   need to call sort_deco directly (but the correctness lemmas should still be useful). *)
-
-fun undecorate_aux :: "'a list \<Rightarrow> 'a sort_key list \<Rightarrow> 'a list" where
-  "undecorate_aux acc [] = rev acc" | "undecorate_aux acc ((_, x) # xs) = undecorate_aux (x # acc) xs"
-
-definition undecorate :: "'a sort_key list \<Rightarrow> 'a list" where
-  "undecorate = undecorate_aux []"
-
-case_of_simps undecorate_aux_eq : undecorate_aux.simps
-function_compile_nat undecorate_aux_eq
-function_compile_nat undecorate_def
 
 end
 
@@ -279,8 +195,6 @@ HOL_To_IMP_Minus_correct GT_nat by cook
 
 section\<open>Comparison (nat)\<close>
 
-find_theorems "case (?x :: nat) of (0) \<Rightarrow> _ | (Suc n) \<Rightarrow> _" "if ?x = 0 then _ else _"
-
 lemmas leq_aux_nat_eq = HOL_To_HOL_Nat.leq_aux_nat_eq_unfolded[simplified case_nat_eq_if]
 unconditional_nat leq_aux_nat_eq
 declare leq_aux_nat_unconditional.simps [simp del]
@@ -289,7 +203,6 @@ HOL_To_IMP_Minus_correct leq_aux_nat_unconditional by (cook mode = tailcall)
 
 unconditional_nat HOL_To_HOL_Nat.leq_eq_leq_aux
 declare less_eq_unconditional.simps [simp del]
-(* TODO: uses helper function *)
 (* compile_nat less_eq_unconditional.simps *)
 (* HOL_To_IMP_Minus_correct less_eq_unconditional by cook *)
 
@@ -305,7 +218,7 @@ HOL_To_IMP_Minus_correct Some_nat by cook
 
 paragraph \<open>is_some\<close>
 
-lemmas is_some_nat_eq = HOL_To_HOL_Nat.is_some_nat_eq_unfolded[simplified case_my_option_nat_def]
+lemmas is_some_nat_eq = HOL_To_HOL_Nat.is_some_nat_eq_unfolded[simplified case_option_nat_def]
 unconditional_nat is_some_nat_eq
 declare is_some_nat_unconditional.simps [simp del]
 compile_nat is_some_nat_unconditional.simps
@@ -313,7 +226,7 @@ HOL_To_IMP_Minus_correct is_some_nat_unconditional by cook
 
 paragraph \<open>get_some\<close>
 
-lemmas get_some_nat_eq = HOL_To_HOL_Nat.get_some_nat_eq_unfolded[simplified case_my_option_nat_def]
+lemmas get_some_nat_eq = HOL_To_HOL_Nat.get_some_nat_eq_unfolded[simplified case_option_nat_def]
 unconditional_nat get_some_nat_eq
 declare get_some_nat_unconditional.simps [simp del]
 compile_nat get_some_nat_unconditional.simps
@@ -336,9 +249,8 @@ declare length_aux_nat_unconditional.simps [simp del]
 compile_nat length_aux_nat_unconditional.simps
 HOL_To_IMP_Minus_correct length_aux_nat_unconditional by (cook mode = tailcall)
 
-(* TODO: this ends up getting named size_... *)
+(* TODO: this ends up getting named size_* *)
 lemmas length_nat_eq = HOL_To_HOL_Nat.size_nat_eq_unfolded[simplified case_list_nat_def]
-(* TODO: uses helper function *)
 (* unconditional_nat length_nat_eq *)
 (* declare length_nat_unconditional.simps [simp del] *)
 (* compile_nat length_nat_unconditional.simps *)
@@ -354,22 +266,22 @@ compile_nat compare_lengths_nat_unconditional.simps
 HOL_To_IMP_Minus_correct compare_lengths_nat_unconditional by (cook mode = tailcall)
 
 
-paragraph \<open>rev_append\<close>
+paragraph \<open>rev_aux\<close>
 
-lemmas rev_append_nat_eq = HOL_To_HOL_Nat.rev_append_nat_eq_unfolded[simplified case_list_nat_def]
-unconditional_nat rev_append_nat_eq
-declare rev_append_nat_unconditional.simps [simp del]
-compile_nat rev_append_nat_unconditional.simps
-HOL_To_IMP_Minus_correct rev_append_nat_unconditional by (cook mode = tailcall)
+lemmas rev_aux_nat_eq = HOL_To_HOL_Nat.rev_aux_nat_eq_unfolded[simplified case_list_nat_def]
+unconditional_nat rev_aux_nat_eq
+declare rev_aux_nat_unconditional.simps [simp del]
+compile_nat rev_aux_nat_unconditional.simps
+HOL_To_IMP_Minus_correct rev_aux_nat_unconditional by (cook mode = tailcall)
 
 paragraph \<open>rev\<close>
 
-(* TODO: can't do functions with helpers! *)
+(* TODO: aux function rev_aux needed for rev *)
 
 
 paragraph \<open>append\<close>
 
-(* TODO: aux function *)
+(* TODO: aux function rev_aux needed for append *)
 
 
 paragraph \<open>zip\<close>
@@ -380,7 +292,7 @@ declare zip_aux_nat_unconditional.simps [simp del]
 compile_nat zip_aux_nat_unconditional.simps
 HOL_To_IMP_Minus_correct zip_aux_nat_unconditional by (cook mode = tailcall)
 
-(* TODO: zip: aux function needed *)
+(* TODO: aux function rev needed for zip *)
 
 
 subsection \<open>Association Lists\<close>
@@ -390,12 +302,6 @@ unconditional_nat assoc_lookup_nat_eq
 declare assoc_lookup_nat_unconditional.simps [simp del]
 compile_nat assoc_lookup_nat_unconditional.simps
 HOL_To_IMP_Minus_correct assoc_lookup_nat_unconditional by (cook mode = tailcall)
-
-
-subsection \<open>Sorting\<close>
-
-(* TODO: get compiling to Nat first *)
-
 
 end
 
